Make HReduce work over any length. Block size is arbitrary

test/Test_Klas_HReduce__U32Plus.cu
@@ -7,42 +7,77 @@ bool ok = true;
 
 /* It would be nicer to write a purely-Pulse test. */
 
-void test(int siz)
-{
-    uint32_t *a;
-    uint32_t *ga;
+#define TYPE uint32_t
+#define FUN  Klas_HReduce_reduce_u32_plus
+#define PR   "%" PRIu32
 
-    a = (uint32_t *) malloc(siz * sizeof a[0]);
-    ga = (uint32_t *) KPR_GPU_ALLOC(sizeof ga[0], siz);
+void test(int nth, int siz)
+{
+    TYPE *a;
+    TYPE *ga;
+
+    a = (TYPE *)malloc(siz * sizeof a[0]);
+    ga = (TYPE *)KPR_GPU_ALLOC(sizeof ga[0], siz);
 
     int i;
 
     for (i = 0; i < siz; i++)
         a[i] = i;
 
-    MUST(cudaMemcpy(ga, a, siz * sizeof(uint32_t), cudaMemcpyHostToDevice));
+    MUST(cudaMemcpy(ga, a, siz * sizeof(TYPE), cudaMemcpyHostToDevice));
 
-    uint32_t res = Klas_HReduce_reduce_u32_plus(siz, ga);
+    TYPE res = FUN(nth, siz, ga);
 
-    MUST(cudaMemcpy(a, ga, siz * sizeof(uint32_t), cudaMemcpyDeviceToHost));
+    MUST(cudaMemcpy(a, ga, siz * sizeof(TYPE), cudaMemcpyDeviceToHost));
     MUST(cudaFree(ga));
 
-    printf("%" PRIu32 "\n", res);
+    // Note: assuming no FP error
     if (res != siz * (siz - 1) / 2)
         ok = false;
+    printf("test(%d, %d) = " PR "%s\n", nth, siz, res, ok ? "" : " (FAILED)");
     free(a);
 }
 
 int main()
 {
-    test(510);
-    test(511);
-    test(512);
-    test(513);
-    test(514);
-    test(1022);
-    test(1023);
-    test(1024);
+    /* Tests with full blocks. */
+    test(1024, 510);
+    test(1024, 511);
+    test(1024, 512);
+    test(1024, 513);
+    test(1024, 514);
+    test(1024, 1022);
+    test(1024, 1023);
+    test(1024, 1024);
+    test(1024, 1025);
+    test(1024, 2048);
+    test(1024, 2049);
+
+    /* Smaller blocks */
+    test(512, 510);
+    test(512, 511);
+    test(512, 512);
+    test(512, 513);
+    test(512, 514);
+    test(512, 1022);
+    test(512, 1023);
+    test(512, 1024);
+    test(512, 1025);
+    test(512, 2048);
+
+    /* Weird sizes */
+    test(1, 0);
+    test(1, 1);
+    test(1, 2);
+    test(2, 0);
+    test(2, 1);
+    test(2, 2);
+    test(3, 0);
+    test(3, 1);
+    test(3, 2);
+    test(4, 0);
+    test(4, 1);
+    test(4, 2);
 
     return !ok;
 }
