src/lib/kernel/Kuiper.Kernel.HReduce.fsti
@@ -4,6 +4,7 @@ module Kuiper.Kernel.HReduce
 
 open Kuiper
 open Kuiper.Tensor { ctlayout }
+module SZ = Kuiper.SizeT
 module Array1 = Kuiper.Array1
 
 // TODO: generalize operation? It currently always uses `add`
@@ -11,16 +12,18 @@ module Array1 = Kuiper.Array1
 
 inline_for_extraction noextract
 type reduce_ty (et : Type0) {| scalar et, real_like et |} =
-  fn (len : szp { len <= max_threads })
-     (#l : Array1.layout len) {| ctlayout l |}
+  fn (nth : szp { nth <= max_threads })
+     (lena : sz)
+     (#l : Array1.layout lena) {| ctlayout l |}
      (a : Array1.t et l { Array1.is_global a })
-     (#va : erased (lseq et len))
-     (vr : erased (lseq real len))
+     (#va : erased (lseq et lena))
+     (vr : erased (lseq real lena))
   preserves
     cpu **
     on gpu_loc (a |-> va)
   requires
-    pure (va %~ vr)
+    pure (va %~ vr) **
+    pure (SZ.fits (lena + nth)) // Almost impossible to falsify
   returns
     res : et
   ensures
