src/lib/kernel/Kuiper.Kernel.Softmax.fst
@@ -57,7 +57,7 @@ fn softmax_gpu
 
   Classical.forall_intro_2 (fun x -> Classical.move_requires (exp_approx #et x));
 
-  let sum = Kuiper.Kernel.HReduce.reduce lena a' (seq_map rexp ra);
+  let sum = Kuiper.Kernel.HReduce.reduce lena lena a' (seq_map rexp ra);
   Array1.free a';
 
   (* Divide by sum *)
